***NO_CI***, stsep specs

examples/seplogic/Lang.fst
@@ -9,6 +9,8 @@ open FStar.Seq
 open FStar.ST
 open FStar.Heap  //this order of opening the modules is important, we want ref from FStar.Heap
 
+open FStar.Tactics
+
 #set-options "--lax"
 
 type addr = ref int
@@ -74,81 +76,35 @@ let rec wp_command (#a:Type0) (c:command a) (p:st_post a) (h0:heap) :Type0
     | Alloc            -> (forall (r:ref int) (h1:heap). (fresh r h0 h1 /\ modifies !{} h0 h1 /\ sel h1 r == 0) ==> p r h1)
     //| Free r           -> False
 
-(* get the nice x <-- c1; c2 syntax *)
-let bind (#a:Type0) (#b:Type0) (c1:command a) (c2:a -> command b) :command b = Bind c1 c2
+let disjoint_partitions (h:heap) (h1:heap) (h2:heap) :Type0 = disjoint h1 h2 /\ h == h1 `join` h2
 
-let distinct_and_contained (r1:addr) (r2:addr) (r3:addr) (r4:addr) (r5:addr) (r6:addr) (h:heap)
-  = addr_of r1 <> addr_of r2 /\ addr_of r1 <> addr_of r3 /\ addr_of r1 <> addr_of r4 /\ addr_of r1 <> addr_of r5 /\ addr_of r1 <> addr_of r6 /\
-    addr_of r2 <> addr_of r3 /\ addr_of r2 <> addr_of r4 /\ addr_of r2 <> addr_of r5 /\ addr_of r2 <> addr_of r6 /\
-    addr_of r3 <> addr_of r4 /\ addr_of r3 <> addr_of r5 /\ addr_of r3 <> addr_of r6 /\
-    addr_of r4 <> addr_of r5 /\ addr_of r4 <> addr_of r6 /\
-    addr_of r5 <> addr_of r6 /\
-    h `contains` r1 /\ h `contains` r2 /\ h `contains` r3 /\ h `contains` r4 /\ h `contains` r5 /\ h `contains` r6
+let rec wpsep_command (#a:Type0) (c:command a) :st_wp a
+  = match c with
+    | Return #a x      -> fun p h0 -> h0 == emp /\ p x h0
 
-let c1 (r1:addr) (n1:int)
-       (r2:addr) (n2:int)
-       (r3:addr) (n3:int)
-       (r4:addr) (n4:int)
-       (r5:addr) (n5:int)
-       (r6:addr) (n6:int)
-  :command int
-  = Write r1 n1;;
-    n <-- Read r1;
-    r <-- Alloc;
-    Write r2 n2;;
-    Write r3 n3;;
-    Write r4 n4;;
-    Write r5 n5;;
-    Write r6 n6;;
-    Write r n1;;
-    Write r1 (n + 1);;
-    n <-- Read r1;
-    r <-- Alloc;
-    Write r2 n6;;
-    Write r3 n5;;
-    Write r4 n4;;
-    Write r5 n5;;
-    Write r6 n6;;
-    Write r n5;;
-    Write r1 (n + 1);;
-    n <-- Read r1;
-    r <-- Alloc;
-    Write r2 n2;;
-    Write r3 n3;;
-    Write r4 n4;;
-    Write r5 n5;;
-    Write r6 n6;;
-    Write r n3;;
-    Write r1 (n + 1);;
-    n <-- Read r1;
-    r <-- Alloc;
-    Write r2 n6;;
-    Write r3 n5;;
-    Write r4 n4;;
-    Write r5 n5;;
-    Write r6 n6;;
-    Write r n5;;
-    Write r1 (n + 1);;
-    n <-- Read r1;
-    Write r2 n2;;
-    Write r3 n3;;
-    Write r4 n4;;
-    Write r5 n5;;
-    Write r6 n6;;
-    Write r1 (n + 1);;
-    n <-- Read r1;
-    r <-- Alloc;
-    Write r2 n6;;
-    Write r3 n5;;
-    Write r4 n4;;
-    Write r5 n5;;
-    Write r6 n6;;
-    Write r n1;;
-    Write r1 (n + 1);;
-    Return 0
-  
+    | Bind #a #b c1 c2 ->
+      FStar.Classical.forall_intro (FStar.WellFounded.axiom1 #a #(command b) c2);
+      fun p h3 -> exists (h2' h2'':heap). (disjoint_partitions h3 h2' h2'') /\
+                                  (wp_command c1) (fun x h1 -> exists h1' h1''. (disjoint h1' h1'' /\ disjoint h1 h2'' /\
+			                                                 h1' `join` h1'' == h1 `join` h2'')
+						                      /\ (wp_command (c2 x)) (fun y h2 -> h2 `disjoint` h1'' /\ p y (h2 `join` h1'')) h1') h2'
+      
+
+    | Read r    -> fun p h0 -> (exists x. points_to r x h0) /\ (forall x. points_to r x h0 ==> p x h0)
+
+    | Write r y -> fun p h0 -> (exists x. points_to r x h0) /\ (forall h1. points_to r y h1 ==> p () h1)
+
+    | Alloc     -> fun p h0 -> h0 == emp /\ (forall r h1. points_to r 0 h1 ==> p r h1)
+
+let lift_wpsep (#a:Type0) (wp_sep:st_wp a) :st_wp a
+  = fun p h0 -> exists h0' h0''. disjoint h0' h0'' /\ h0 == h0' `join` h0'' /\
+                         wp_sep (fun x h1' -> disjoint h1' h0'' /\ p x (h1' `join` h0'')) h0'
+
 let steps :list step = [delta_only
   ["Lang.wp_command";
+   "Lang.wpsep_command";
+   "Lang.lift_wpsep";
+   "Lang.disjoint_partitions";
    "Lang.uu___is_Return";
    "Lang.uu___is_Bind";
    "Lang.uu___is_Read";
@@ -166,18 +122,170 @@ let steps :list step = [delta_only
    zeta; iota; primops
   ]
 
-#reset-options
+#reset-options "--z3rlimit 5"
+(* get the nice x <-- c1; c2 syntax *)
+//let bind (#a:Type0) (#b:Type0) (c1:command a) (c2:a -> command b) :command b = Bind c1 c2
 
-#set-options "--z3rlimit 10"
-let foo (r1:addr) (n1:int)
-        (r2:addr) (n2:int)
-        (r3:addr) (n3:int)
-        (r4:addr) (n4:int)
-        (r5:addr) (n5:int)
-        (r6:addr) (n6:int)
-        (h:heap{distinct_and_contained r1 r2 r3 r4 r5 r6 h})
-  =  let p1  :st_post int = fun _ h -> sel h r1 == n1 + 6 /\ sel h r2 == n6 /\ sel h r3 == n5 /\ sel h r4 == n4 /\ sel h r5 == n5 /\ sel h r6 == n6
-     in
+let unfold_fns :list string = [
+  "wp_command"; "wpsep_command"; "lift_wpsep"; "disjoint_partitions"; "uu___is_Return"; "uu___is_Bind";
+  "uu___is_Read"; "uu___is_Write"; "uu___is_Alloc"; "__proj__Return__item__v";
+   "__proj__Bind__item__c1"; "__proj__Bind__item__c2"; "__proj__Read__item__id";
+   "__proj__Write__item__id"; "__proj__Write__item__v"
+  ]
 
-     let t  = wp_command (c1 r1 n1 r2 n2 r3 n3 r4 n4 r5 n5 r6 n6) p1 h in
-     assert (Prims.norm steps t)
+unfold let unfold_steps =
+  List.Tot.map (fun s -> pack_fv ["Lang"; s]) unfold_fns
+
+let foo (r1:addr) (r2:addr) (h:heap{sel h r2 == 4 /\ addr_of r1 <> addr_of r2})
+  = let c = Bind (Write r1 3) (fun _ -> Read r1) in
+    let p :st_post int = fun _ h -> sel h r2 == 4 in
+    let t = (lift_wpsep (wpsep_command c)) p h in
+    assert_by_tactic t (norm [Delta; UnfoldOnly unfold_steps; Primops];; dump "Foo")
+
+
+
+exists h0' h0''. h == h0' `join` h0'' /\
+                 (exists h2' h2''. h0' == h2' `join` h2'' /\
+                                   (forall h1. sel h1 r1 == 3 ==>
+                                               (exists h1' h1''. h1' `join` h1'' == h1 `join` h2'' /\
+                                                                 sel ((h1' `join` h1'') `join` h0'') r2 == 4)))
+
+
+
+
+
+    assert_by_tactic t (norm [Delta; UnfoldOnly [pack_fv ["Lang"; "wp_command"];
+                                                 pack_fv ["Lang"; "wpsep_command"];
+						 pack_fv ["Lang"; "disjoint_partitions"];
+						 pack_fv ["Lang"; "uu___is_Return"];
+						 pack_fv ["Lang"; "uu___is_Bind"];
+						 pack_fv ["Lang"; "uu___is_Read"];
+						 pack_fv ["Lang"; "uu___is_Write"];
+						 pack_fv ["Lang"; "uu___is_Alloc"];
+						 pack_fv ["Lang"; "__proj__Return__item__v"];
+						 pack_fv ["Lang"; "__proj__Bind__item__c1"];
+						 pack_fv ["Lang"; "__proj__Bind__item__c2"];
+						 pack_fv ["Lang"; "__proj__Read__item__id"];
+						 pack_fv ["Lang"; "__proj__Write__item__id"];
+						 pack_fv ["Lang"; "__proj__Write__item__v"];
+						 ];
+			      Primops])
+
+(* #set-options "--z3rlimit 10" *)
+(* let foo (r1:addr) (n1:int) *)
+(*         (r2:addr) (n2:int) *)
+(*         (r3:addr) (n3:int) *)
+(*         (r4:addr) (n4:int) *)
+(*         (r5:addr) (n5:int) *)
+(*         (r6:addr) (n6:int) *)
+(*         (h:heap{distinct_and_contained r1 r2 r3 r4 r5 r6 h}) *)
+(*   =  let p1  :st_post int = fun _ h -> sel h r1 == n1 + 6 /\ sel h r2 == n6 /\ sel h r3 == n5 /\ sel h r4 == n4 /\ sel h r5 == n5 /\ sel h r6 == n6 *)
+(*      in *)
+
+(*      let t  = wp_command (c1 r1 n1 r2 n2 r3 n3 r4 n4 r5 n5 r6 n6) p1 h in *)
+(*      assert (Prims.norm steps t) *)
+
+(* (\* let distinct_and_contained (r1:addr) (r2:addr) (r3:addr) (r4:addr) (r5:addr) (r6:addr) (h:heap) *\) *)
+(* (\*   = addr_of r1 <> addr_of r2 /\ addr_of r1 <> addr_of r3 /\ addr_of r1 <> addr_of r4 /\ addr_of r1 <> addr_of r5 /\ addr_of r1 <> addr_of r6 /\ *\) *)
+(* (\*     addr_of r2 <> addr_of r3 /\ addr_of r2 <> addr_of r4 /\ addr_of r2 <> addr_of r5 /\ addr_of r2 <> addr_of r6 /\ *\) *)
+(* (\*     addr_of r3 <> addr_of r4 /\ addr_of r3 <> addr_of r5 /\ addr_of r3 <> addr_of r6 /\ *\) *)
+(* (\*     addr_of r4 <> addr_of r5 /\ addr_of r4 <> addr_of r6 /\ *\) *)
+(* (\*     addr_of r5 <> addr_of r6 /\ *\) *)
+(* (\*     h `contains` r1 /\ h `contains` r2 /\ h `contains` r3 /\ h `contains` r4 /\ h `contains` r5 /\ h `contains` r6 *\) *)
+
+(* (\* let c1 (r1:addr) (n1:int) *\) *)
+(* (\*        (r2:addr) (n2:int) *\) *)
+(* (\*        (r3:addr) (n3:int) *\) *)
+(* (\*        (r4:addr) (n4:int) *\) *)
+(* (\*        (r5:addr) (n5:int) *\) *)
+(* (\*        (r6:addr) (n6:int) *\) *)
+(* (\*   :command int *\) *)
+(* (\*   = Write r1 n1;; *\) *)
+(* (\*     n <-- Read r1; *\) *)
+(* (\*     r <-- Alloc; *\) *)
+(* (\*     Write r2 n2;; *\) *)
+(* (\*     Write r3 n3;; *\) *)
+(* (\*     Write r4 n4;; *\) *)
+(* (\*     Write r5 n5;; *\) *)
+(* (\*     Write r6 n6;; *\) *)
+(* (\*     Write r n1;; *\) *)
+(* (\*     Write r1 (n + 1);; *\) *)
+(* (\*     n <-- Read r1; *\) *)
+(* (\*     r <-- Alloc; *\) *)
+(* (\*     Write r2 n6;; *\) *)
+(* (\*     Write r3 n5;; *\) *)
+(* (\*     Write r4 n4;; *\) *)
+(* (\*     Write r5 n5;; *\) *)
+(* (\*     Write r6 n6;; *\) *)
+(* (\*     Write r n5;; *\) *)
+(* (\*     Write r1 (n + 1);; *\) *)
+(* (\*     n <-- Read r1; *\) *)
+(* (\*     r <-- Alloc; *\) *)
+(* (\*     Write r2 n2;; *\) *)
+(* (\*     Write r3 n3;; *\) *)
+(* (\*     Write r4 n4;; *\) *)
+(* (\*     Write r5 n5;; *\) *)
+(* (\*     Write r6 n6;; *\) *)
+(* (\*     Write r n3;; *\) *)
+(* (\*     Write r1 (n + 1);; *\) *)
+(* (\*     n <-- Read r1; *\) *)
+(* (\*     r <-- Alloc; *\) *)
+(* (\*     Write r2 n6;; *\) *)
+(* (\*     Write r3 n5;; *\) *)
+(* (\*     Write r4 n4;; *\) *)
+(* (\*     Write r5 n5;; *\) *)
+(* (\*     Write r6 n6;; *\) *)
+(* (\*     Write r n5;; *\) *)
+(* (\*     Write r1 (n + 1);; *\) *)
+(* (\*     n <-- Read r1; *\) *)
+(* (\*     Write r2 n2;; *\) *)
+(* (\*     Write r3 n3;; *\) *)
+(* (\*     Write r4 n4;; *\) *)
+(* (\*     Write r5 n5;; *\) *)
+(* (\*     Write r6 n6;; *\) *)
+(* (\*     Write r1 (n + 1);; *\) *)
+(* (\*     n <-- Read r1; *\) *)
+(* (\*     r <-- Alloc; *\) *)
+(* (\*     Write r2 n6;; *\) *)
+(* (\*     Write r3 n5;; *\) *)
+(* (\*     Write r4 n4;; *\) *)
+(* (\*     Write r5 n5;; *\) *)
+(* (\*     Write r6 n6;; *\) *)
+(* (\*     Write r n1;; *\) *)
+(* (\*     Write r1 (n + 1);; *\) *)
+(* (\*     Return 0 *\) *)
+  
+(* (\* let steps :list step = [delta_only *\) *)
+(* (\*   ["Lang.wp_command"; *\) *)
+(* (\*    "Lang.uu___is_Return"; *\) *)
+(* (\*    "Lang.uu___is_Bind"; *\) *)
+(* (\*    "Lang.uu___is_Read"; *\) *)
+(* (\*    "Lang.uu___is_Write"; *\) *)
+(* (\*    "Lang.uu___is_Alloc"; *\) *)
+(* (\*    "Lang.__proj__Return__item__v"; *\) *)
+(* (\*    "Lang.__proj__Bind__item__c1"; *\) *)
+(* (\*    "Lang.__proj__Bind__item__c2"; *\) *)
+(* (\*    "Lang.__proj__Read__item__id"; *\) *)
+(* (\*    "Lang.__proj__Write__item__id"; *\) *)
+(* (\*    "Lang.__proj__Write__item__v"; *\) *)
+(* (\*    "Lang.c1"; *\) *)
+(* (\*    "Lang.bind"]; *\) *)
+
+(* (\*    zeta; iota; primops *\) *)
+(* (\*   ] *\) *)
+
+(* (\* #reset-options *\) *)
+
+(* (\* #set-options "--z3rlimit 10" *\) *)
+(* (\* let foo (r1:addr) (n1:int) *\) *)
+(* (\*         (r2:addr) (n2:int) *\) *)
+(* (\*         (r3:addr) (n3:int) *\) *)
+(* (\*         (r4:addr) (n4:int) *\) *)
+(* (\*         (r5:addr) (n5:int) *\) *)
+(* (\*         (r6:addr) (n6:int) *\) *)
+(* (\*         (h:heap{distinct_and_contained r1 r2 r3 r4 r5 r6 h}) *\) *)
+(* (\*   =  let p1  :st_post int = fun _ h -> sel h r1 == n1 + 6 /\ sel h r2 == n6 /\ sel h r3 == n5 /\ sel h r4 == n4 /\ sel h r5 == n5 /\ sel h r6 == n6 *\) *)
+(* (\*      in *\) *)
+
+(* (\*      let t  = wp_command (c1 r1 n1 r2 n2 r3 n3 r4 n4 r5 n5 r6 n6) p1 h in *\) *)
+(* (\*      assert (Prims.norm steps t) *\) *)
